wasm: Improve naming in wasmBoth

compiler/backend/semantics/wasmBothScript.sml
@@ -5,15 +5,15 @@ val _ = ParseExtras.tight_equality()
 
 val _ = new_theory "wasmBoth"
 
-val state_rel_def = Define `
-  state_rel (rs:'a wasmRelSem$state) (fs:'a wasmSem$state) <=>
+val states_agree_def = Define `
+  states_agree (rs:'a wasmRelSem$state) (fs:'a wasmSem$state) <=>
     rs.ffi   = fs.ffi   /\
     rs.store = fs.store /\
     rs.frame = fs.frame /\
     rs.code  = fs.code`
 
-val to_small_state_def = Define `
-  to_small_state (s:'a wasmSem$state) =
+val to_rel_state_def = Define `
+  to_rel_state (s:'a wasmSem$state) =
     <| ffi    := s.ffi
      ; store  := s.store
      ; frame  := s.frame
@@ -21,16 +21,16 @@ val to_small_state_def = Define `
      ; result := NONE
      |>`
 
-val to_small_state_rel = Q.store_thm("to_small_state_rel",
-  `∀s. state_rel (to_small_state s) s`,
-  rw[state_rel_def, to_small_state_def]
+val to_rel_state_agrees = Q.store_thm("to_rel_state_agrees",
+  `∀s. states_agree (to_rel_state s) s`,
+  rw[states_agree_def, to_rel_state_def]
 )
 
-val small_to_big = Q.store_thm("small_to_big",
-  `(∀r s s'.
+val relsem_to_sem = Q.store_thm("relsem_to_sem",
+  `(∀s s' r.
       (evaluate_wasm s = (r, s') ∧ r ≠ Timeout)
     ⇒
-      (∃x. (to_small_state s) --->* x ∧ state_rel x s' ∧ x.result = (SOME r))
+      (∃x. (to_rel_state s) --->* x ∧ state_rel x s' ∧ x.result = (SOME r))
    )`,
   cheat
 )
